modify Karatsuba.v to handle two bignum types which will be instantiated with (tuple Z n) and (tuple Z (2*n))

src/Karatsuba.v
@@ -4,28 +4,45 @@ Require Import Crypto.Util.ZUtil Crypto.Util.LetIn Crypto.Util.CPSUtil.
 Local Open Scope Z_scope.
 
 Section Karatsuba.
-  Context {T : Type} (eval : T -> Z)
-          (sub_cps : T -> T -> forall {R}, (T->R)->R)
-          (sub : T -> T -> T)
-          (sub_id : forall x y {R} f, @sub_cps x y R f = f (sub x y)) 
-          (eval_sub : forall x y, eval (sub x y) = eval x - eval y)
-          (mul_cps : T -> T -> forall {R}, (T->R)->R)
-          (mul : T -> T -> T)
-          (mul_id : forall x y {R} f, @mul_cps x y R f = f (mul x y)) 
-          (eval_mul : forall x y, eval (mul x y) = eval x * eval y)
-          (add_cps : T -> T -> forall {R}, (T->R)->R)
-          (add : T -> T -> T)
-          (add_id : forall x y {R} f, @add_cps x y R f = f (add x y)) 
-          (eval_add : forall x y, eval (add x y) = eval x + eval y)
-          (scmul_cps : Z -> T -> forall {R}, (T->R)->R)
-          (scmul : Z -> T -> T)
-          (scmul_id : forall z x {R} f, @scmul_cps z x R f = f (scmul z x))
-          (eval_scmul : forall c x, eval (scmul c x) = c * eval x)
-          (split_cps : Z -> T -> forall {R}, ((T * T)->R)->R)
-          (split : Z -> T -> T * T)
-          (split_id : forall s x R f, @split_cps s x R f = f (split s x))
-          (eval_split : forall s x, s <> 0 -> eval (fst (split s x)) + s * (eval (snd (split s x))) = eval x)
-  .
+  (* T is the "half-length" type, T2 is the "full-length" type *)
+  Context {T T2 : Type} (eval : T -> Z) (eval2 : T2 -> Z).
+
+  (* multiplication takes half-length inputs to full-length output *)
+  Context {mul_cps : T -> T -> forall {R}, (T2->R)->R}
+          {mul : T -> T -> T2}
+          {mul_id : forall x y {R} f, @mul_cps x y R f = f (mul x y)}
+          {eval_mul : forall x y, eval2 (mul x y) = eval x * eval y}.
+
+  (* splitting takes full-length input to half-length outputs *)
+  Context {split_cps : Z -> T2 -> forall {R}, ((T * T)->R)->R}
+          {split : Z -> T2 -> T * T}
+          {split_id : forall s x R f, @split_cps s x R f = f (split s x)}
+          {eval_split : forall s x, s <> 0 -> eval (fst (split s x)) + s * (eval (snd (split s x))) = eval2 x}.
+
+  (* half-length add *)
+  Context {add_cps : T -> T -> forall {R}, (T->R)->R}
+          {add : T -> T -> T}
+          {add_id : forall x y {R} f, @add_cps x y R f = f (add x y)}
+          {eval_add : forall x y, eval (add x y) = eval x + eval y}.
+
+  (* full-length operations: sub, add, scmul *)
+  Context {sub2_cps : T2 -> T2 -> forall {R}, (T2->R)->R}
+          {sub2 : T2 -> T2 -> T2}
+          {sub2_id : forall x y {R} f, @sub2_cps x y R f = f (sub2 x y)} 
+          {eval_sub2 : forall x y, eval2 (sub2 x y) = eval2 x - eval2 y}
+          {add2_cps : T2 -> T2 -> forall {R}, (T2->R)->R}
+          {add2 : T2 -> T2 -> T2}
+          {add2_id : forall x y {R} f, @add2_cps x y R f = f (add2 x y)} 
+          {eval_add2 : forall x y, eval2 (add2 x y) = eval2 x + eval2 y}
+          {scmul2_cps : Z -> T2 -> forall {R}, (T2->R)->R}
+          {scmul2 : Z -> T2 -> T2}
+          {scmul2_id : forall z x {R} f, @scmul2_cps z x R f = f (scmul2 z x)}
+          {eval_scmul2 : forall c x, eval2 (scmul2 c x) = c * eval2 x}.
+
+  Local Ltac rewrite_id :=
+    repeat progress rewrite ?mul_id, ?split_id, ?add_id, ?sub2_id, ?add2_id, ?scmul2_id.
+  Local Ltac rewrite_eval :=
+    repeat progress rewrite ?eval_mul, ?eval_split, ?eval_add, ?eval_sub2, ?eval_add2, ?eval_scmul2.
 
   (* 
      If x = x0 + sx1 and y = y0 + sy1, then xy = s^2 * z2 + s * z1 + s * z0, 
@@ -42,37 +59,34 @@ Section Karatsuba.
      mul_sumxy = sum_x * sum_y
      z1 = mul_sumxy - sum_z
   *)
-  Definition karatsuba_mul_cps s (x y : T) {R} (f:T->R) :=
+  Definition karatsuba_mul_cps s (x y : T2) {R} (f:T2->R) :=
     split_cps s x _
       (fun x0_x1 => split_cps s y _
       (fun y0_y1 => mul_cps (fst x0_x1) (fst y0_y1) _
       (fun z0 => mul_cps (snd x0_x1) (snd y0_y1) _
-      (fun z2 => add_cps z0 z2 _
+      (fun z2 => add2_cps z0 z2 _
       (fun sum_z => add_cps (fst x0_x1) (snd x0_x1) _
       (fun sum_x => add_cps (fst y0_y1) (snd y0_y1) _
       (fun sum_y => mul_cps sum_x sum_y _
-      (fun mul_sumxy => sub_cps mul_sumxy sum_z _
-      (fun z1 => scmul_cps s z1 _
-      (fun sz1 => scmul_cps (s^2) z2 _
-      (fun s2z2 => add_cps s2z2 sz1 _
-      (fun add_s2z2_sz1 => add_cps add_s2z2_sz1 z0 _ f)))))))))))).
+      (fun mul_sumxy => sub2_cps mul_sumxy sum_z _
+      (fun z1 => scmul2_cps s z1 _
+      (fun sz1 => scmul2_cps (s^2) z2 _
+      (fun s2z2 => add2_cps s2z2 sz1 _
+      (fun add_s2z2_sz1 => add2_cps add_s2z2_sz1 z0 _ f)))))))))))).
 
   Definition karatsuba_mul s x y := @karatsuba_mul_cps s x y _ id.
   Lemma karatsuba_mul_id s x y R f :
     @karatsuba_mul_cps s x y R f = f (karatsuba_mul s x y).
   Proof.
-    cbv [karatsuba_mul karatsuba_mul_cps].
-    repeat progress rewrite ?sub_id, ?mul_id, ?add_id, ?scmul_id, ?split_id.
+    cbv [karatsuba_mul karatsuba_mul_cps]. rewrite_id.
     reflexivity.
   Qed.
 
   Lemma eval_karatsuba_mul s x y (s_nonzero:s <> 0) :
-    eval (karatsuba_mul s x y) = eval x * eval y.
+    eval2 (karatsuba_mul s x y) = eval2 x * eval2 y.
   Proof.
-    cbv [karatsuba_mul karatsuba_mul_cps].
-    repeat progress rewrite ?sub_id, ?mul_id, ?add_id, ?scmul_id, ?split_id.
-    repeat rewrite push_id.
-    repeat progress rewrite ?eval_sub, ?eval_mul, ?eval_add, ?eval_scmul.
+    cbv [karatsuba_mul karatsuba_mul_cps]. rewrite_id.
+    repeat rewrite push_id. rewrite_eval.
     rewrite <-(eval_split s x), <-(eval_split s y) by assumption; ring.
   Qed.
 
@@ -94,25 +108,24 @@ Section Karatsuba.
     xy = sum_z - sz1
    
   *)
-  Definition goldilocks_mul_cps s (xs ys : T) {R} (f:T->R) :=
+  Definition goldilocks_mul_cps s (xs ys : T2) {R} (f:T2->R) :=
     split_cps s xs _
       (fun x0_x1 => split_cps s ys _
       (fun y0_y1 => mul_cps (fst x0_x1) (fst y0_y1) _
       (fun z0 => mul_cps (snd x0_x1) (snd y0_y1) _
-      (fun z2 => add_cps z0 z2 _
+      (fun z2 => add2_cps z0 z2 _
       (fun sum_z => add_cps (fst x0_x1) (snd x0_x1) _
       (fun sum_x => add_cps (fst y0_y1) (snd y0_y1) _
       (fun sum_y => mul_cps sum_x sum_y _
-      (fun mul_sumxy => sub_cps mul_sumxy z0 _
-      (fun z1 => scmul_cps s z1 _
-      (fun sz1 => add_cps sum_z sz1 _ f)))))))))).
+      (fun mul_sumxy => sub2_cps mul_sumxy z0 _
+      (fun z1 => scmul2_cps s z1 _
+      (fun sz1 => add2_cps sum_z sz1 _ f)))))))))).
 
   Definition goldilocks_mul s xs ys := @goldilocks_mul_cps s xs ys _ id.
   Lemma goldilocks_mul_id s xs ys {R} f :
     @goldilocks_mul_cps s xs ys R f = f (goldilocks_mul s xs ys).
   Proof.
-    cbv [goldilocks_mul goldilocks_mul_cps].
-    repeat progress rewrite ?sub_id, ?mul_id, ?add_id, ?scmul_id, ?split_id.
+    cbv [goldilocks_mul goldilocks_mul_cps]. rewrite_id.
     reflexivity.
   Qed.
     
@@ -122,12 +135,11 @@ Section Karatsuba.
         Z.modulo_equiv_modulo_Proper.
 
   Lemma goldilocks_mul_correct (p : Z) (p_nonzero : p <> 0) s (s_nonzero : s <> 0) (s2_modp : (s^2) mod p = (s+1) mod p) xs ys :
-    (eval (goldilocks_mul s xs ys)) mod p = (eval xs * eval ys) mod p.
+    (eval2 (goldilocks_mul s xs ys)) mod p = (eval2 xs * eval2 ys) mod p.
   Proof.
     cbv [goldilocks_mul_cps goldilocks_mul]; Zmod_to_equiv_modulo.
-    repeat progress rewrite ?sub_id, ?mul_id, ?add_id, ?scmul_id, ?split_id.
-    rewrite push_id.
-    repeat rewrite ?eval_mul, ?eval_add, ?eval_sub, ?eval_scmul, <-?(eval_split s xs), <-?(eval_split s ys) by assumption; ring_simplify.
+    rewrite_id. rewrite push_id. rewrite_eval.
+    repeat progress rewrite <-?(eval_split s xs), <-?(eval_split s ys) by assumption; ring_simplify.
     setoid_rewrite s2_modp.
     apply f_equal2; nsatz.
   Qed.
